verified/sec_prop_entry.i.dfy
@@ -1,0 +1,563 @@
+include "sec_prop.s.dfy"
+include "pagedb.s.dfy"
+include "entry.s.dfy"
+include "sec_prop_util.i.dfy"
+include "smcapi.i.dfy"
+
+lemma lemma_enter_enc_conf_ni(s1: state, d1: PageDb, s1':state, d1': PageDb,
+                              s2: state, d2: PageDb, s2':state, d2': PageDb,
+                              dispPage: word, arg1: word, arg2: word, arg3: word,
+                              atkr: PageNr)
+    requires ni_reqs(s1, d1, s1', d1', s2, d2, s2', d2', atkr)
+    requires smc_enter(s1, d1, s1', d1', dispPage, arg1, arg2, arg3)
+    requires smc_enter(s2, d2, s2', d2', dispPage, arg1, arg2, arg3)
+    requires enc_conf_eqpdb(d1, d2, atkr)
+    requires entering_atkr(d1, d2, dispPage, atkr, false) ==>
+        enc_conf_eq_entry(s1, s2, d1, d2, atkr)
+    ensures enc_conf_eqpdb(d1', d2', atkr)
+    ensures entering_atkr(d1, d2, dispPage, atkr, false) ==>
+        enc_conf_eq_entry(s1', s2', d1', d2', atkr)
+{
+    reveal_enc_conf_eqpdb();
+    if(!validPageNr(dispPage)){
+        assert d1' == d1 &&  d2' == d2;
+    } else {
+        assert d1[dispPage].PageDbEntryFree? <==> d2[dispPage].PageDbEntryFree?;
+        if(d1[dispPage].PageDbEntryFree?) {
+            assert d1' == d1 &&  d2' == d2;
+        } else {
+            assert d2[dispPage].PageDbEntryTyped?;
+            var asp1, asp2 := d1[dispPage].addrspace, d2[dispPage].addrspace;
+            var e1', e2' := smc_enter_err(d1, dispPage, false), smc_enter_err(d2, dispPage, false);
+            assert enc_conf_eqpdb(d1', d2', atkr) by {
+                lemma_enter_enc_conf_eqpdb(s1, d1, s1', d1', s2, d2, s2', d2',
+                                 dispPage, arg1, arg2, arg3, asp1, asp2, atkr);
+            }
+            assert pgInAddrSpc(d1, dispPage, atkr) <==>
+                pgInAddrSpc(d2, dispPage, atkr);
+            assert pgInAddrSpc(d1, dispPage, atkr) ==>
+                d1[dispPage].addrspace == atkr;
+            assert pgInAddrSpc(d1, dispPage, atkr) ==>
+                d1[dispPage].addrspace == atkr;
+            assert asp1 == atkr <==> asp2 == atkr;
+
+            if(asp1 == atkr) {
+                assert e1' == KOM_ERR_SUCCESS <==> e2' == KOM_ERR_SUCCESS;
+                if(e1' == KOM_ERR_SUCCESS) {
+                    assert entering_atkr(d1, d2, dispPage, atkr, false);
+                    lemma_enter_enc_conf_atkr_enter(s1, d1, s1', d1', s2, d2, s2', d2',
+                                                    dispPage, arg1, arg2, arg3, 
+                                                    atkr);
+                    assert enc_conf_eq_entry(s1', s2', d1', d2', atkr);
+                } else {
+                    assert !entering_atkr(d1, d2, dispPage, atkr, false);
+                }
+            } else {
+                assert !entering_atkr(d1, d2, dispPage, atkr, false);
+            }
+        }
+    }
+}
+
+lemma lemma_enter_enc_conf_eqpdb(s1: state, d1: PageDb, s1':state, d1': PageDb,
+                                 s2: state, d2: PageDb, s2':state, d2': PageDb,
+                                 disp: word, arg1: word, arg2: word, arg3: word,
+                                 asp1: PageNr, asp2: PageNr, atkr: PageNr)
+    requires ni_reqs(s1, d1, s1', d1', s2, d2, s2', d2', atkr)
+    requires smc_enter(s1, d1, s1', d1', disp, arg1, arg2, arg3)
+    requires smc_enter(s2, d2, s2', d2', disp, arg1, arg2, arg3)
+    requires validPageNr(disp) && d1[disp].PageDbEntryTyped? && 
+        d2[disp].PageDbEntryTyped?
+    requires d1[disp].addrspace == asp1 && d2[disp].addrspace == asp2
+    requires enc_conf_eqpdb(d1, d2, atkr)
+    requires entering_atkr(d1, d2, disp, atkr, false) ==>
+        enc_conf_eq_entry(s1, s2, d1, d2, atkr)
+    ensures  enc_conf_eqpdb(d1', d2', atkr)
+{
+
+    reveal_enc_conf_eqpdb();
+    var go1 := smc_enter_err(d1, disp, false) == KOM_ERR_SUCCESS;
+    var go2 := smc_enter_err(d2, disp, false) == KOM_ERR_SUCCESS;
+
+    if(go1 && go2) {
+        lemma_enter_only_affects_entered(s1, d1, s1', d1',
+             disp, asp1, arg1, arg2, arg3);
+        lemma_enter_only_affects_entered(s2, d2, s2', d2',
+             disp, asp2, arg1, arg2, arg3);
+        
+        assert d1[atkr].PageDbEntryTyped? <==> d2[atkr].PageDbEntryTyped?;
+        assert d1[atkr].PageDbEntryTyped? <==> d1'[atkr].PageDbEntryTyped?;
+        assert d2[atkr].PageDbEntryTyped? <==> d2'[atkr].PageDbEntryTyped?;
+        assert d1'[atkr].PageDbEntryTyped? <==> d2'[atkr].PageDbEntryTyped?;
+       
+        assert valAddrPage(d1, asp1) && valAddrPage(d2, asp2);
+
+        assert pgInAddrSpc(d1, disp, atkr) <==>
+            pgInAddrSpc(d2, disp, atkr);
+        assert pgInAddrSpc(d1, disp, atkr) ==>
+            d1[disp].addrspace == atkr;
+        assert pgInAddrSpc(d1, disp, atkr) ==>
+            d1[disp].addrspace == atkr;
+        assert asp1 == atkr <==> asp2 == atkr;
+        
+        if(asp1 == atkr) {
+            assert entering_atkr(d1, d2, disp, atkr, false);
+            assert enc_conf_eq_entry(s1, s2, d1, d2, atkr);
+            lemma_enter_enc_conf_atkr_enter(s1, d1, s1', d1', s2, d2, s2', d2',
+                                            disp, arg1, arg2, arg3, 
+                                            atkr);
+        } else {
+            assert asp1 != atkr && asp2 != atkr;
+            assert outside_world_same(d1, d1', disp, asp1);
+            assert outside_world_same(d2, d2', disp, asp2);
+
+            assert forall n : PageNr :: pgInAddrSpc(d1', n, asp1)
+                <==>  pgInAddrSpc(d1, n, asp1);
+            assert forall n : PageNr :: pgInAddrSpc(d1', n, atkr)
+                ==> !pgInAddrSpc(d1', n, asp1);
+
+            assert forall n : PageNr :: pgInAddrSpc(d2', n, asp2)
+                <==>  pgInAddrSpc(d2, n, asp2);
+            assert forall n : PageNr :: pgInAddrSpc(d2', n, atkr)
+                ==> !pgInAddrSpc(d2', n, asp2);
+
+            assert (forall n : PageNr | pgInAddrSpc(d1', n, atkr) 
+                && d1'[n].PageDbEntryTyped? ::
+                    d1'[n].addrspace == d1[n].addrspace &&
+                    d1'[n].entry == d1[n].entry);
+            
+            assert (forall n : PageNr | pgInAddrSpc(d2', n, atkr) 
+                && d2'[n].PageDbEntryTyped? ::
+                    d2'[n].addrspace == d2[n].addrspace &&
+                    d2'[n].entry == d2[n].entry);
+            
+            assert forall n : PageNr :: pgInAddrSpc(d1', n, atkr) <==>
+                pgInAddrSpc(d1, n, atkr);
+            assert forall n : PageNr :: pgInAddrSpc(d2', n, atkr) <==>
+                pgInAddrSpc(d2, n, atkr);
+            assert forall n : PageNr :: pgInAddrSpc(d1', n, atkr) <==>
+                pgInAddrSpc(d2', n, atkr);
+
+            assert forall n : PageNr | pgInAddrSpc(d1', n, atkr) ::
+                d1'[n].entry == d2'[n].entry;
+            
+            assert enc_conf_eqpdb(d1', d2', atkr);
+            
+        }
+    }
+
+    if(go1 && !go2) {
+        lemma_enter_enc_conf_eqpdb_one_go(s1, d1, s1', d1', s2, d2, s2', d2',
+                         disp, arg1, arg2, arg3, asp1, asp2, atkr);
+        assert enc_conf_eqpdb(d1', d2', atkr);
+    }
+    if(!go1 && go2) {
+        lemma_enter_enc_conf_eqpdb_one_go(s2, d2, s2', d2', s1, d1, s1', d1',
+                         disp, arg1, arg2, arg3, asp2, asp1, atkr);
+        assert enc_conf_eqpdb(d1', d2', atkr);
+    }
+    if(!go1 && !go2) { 
+        assert d1' == d1 && d2' == d2;
+        assert enc_conf_eqpdb(d1', d2', atkr);
+    }
+}
+
+lemma lemma_enter_enc_conf_eqpdb_one_go(s1: state, d1: PageDb, s1':state, d1': PageDb,
+                                        s2: state, d2: PageDb, s2':state, d2': PageDb,
+                                        disp: word, arg1: word, arg2: word, arg3: word,
+                                        asp1: PageNr, asp2: PageNr, atkr: PageNr)
+    requires ni_reqs(s1, d1, s1', d1', s2, d2, s2', d2', atkr)
+    requires smc_enter(s1, d1, s1', d1', disp, arg1, arg2, arg3)
+    requires smc_enter(s2, d2, s2', d2', disp, arg1, arg2, arg3)
+    requires validPageNr(disp) && d1[disp].PageDbEntryTyped? && 
+        d2[disp].PageDbEntryTyped?
+    requires d1[disp].addrspace == asp1 && d2[disp].addrspace == asp2
+    requires enc_conf_eqpdb(d1, d2, atkr)
+    requires smc_enter_err(d1, disp, false) == KOM_ERR_SUCCESS
+            && !(smc_enter_err(d2, disp, false) == KOM_ERR_SUCCESS);
+    ensures  enc_conf_eqpdb(d1', d2', atkr)
+{
+   reveal_enc_conf_eqpdb();
+   var go1 := smc_enter_err(d1, disp, false) == KOM_ERR_SUCCESS;
+   var go2 := smc_enter_err(d2, disp, false) == KOM_ERR_SUCCESS;
+   assert go1 && !go2;
+   
+   assert d2' == d2;
+
+   var asp1 := d1[disp].addrspace;
+
+   assert asp1 != atkr by {
+       var asp2 := d2[disp].addrspace;
+       assert pgInAddrSpc(d1, disp, atkr) <==>
+           pgInAddrSpc(d2, disp, atkr);
+       assert pgInAddrSpc(d1, disp, atkr) ==>
+           d1[disp].addrspace == atkr;
+       assert pgInAddrSpc(d1, disp, atkr) ==>
+           d1[disp].addrspace == atkr;
+       assert asp1 == atkr <==> asp2 == atkr;
+       assert asp2 == atkr && go1 ==> go2;
+   }
+
+   lemma_enter_only_affects_entered(s1, d1, s1', d1',
+        disp, asp1, arg1, arg2, arg3);
+   assert outside_world_same(d1, d1', disp, asp1);
+
+   assert forall n : PageNr :: pgInAddrSpc(d1', n, asp1)
+       <==>  pgInAddrSpc(d1, n, asp1);
+   assert forall n : PageNr :: pgInAddrSpc(d1', n, atkr)
+       ==> !pgInAddrSpc(d1', n, asp1);
+
+   assert (forall n : PageNr | pgInAddrSpc(d1', n, atkr) 
+       && d1'[n].PageDbEntryTyped? ::
+           d1'[n].addrspace == d1[n].addrspace &&
+           d1'[n].entry == d1[n].entry);
+   
+   assert forall n : PageNr :: pgInAddrSpc(d1', n, atkr) <==>
+       pgInAddrSpc(d1, n, atkr);
+   assert forall n : PageNr :: pgInAddrSpc(d1', n, atkr) <==>
+       pgInAddrSpc(d2', n, atkr);
+
+   assert forall n : PageNr | pgInAddrSpc(d1', n, atkr) ::
+       d1'[n].entry == d2'[n].entry;
+   
+   assert enc_conf_eqpdb(d1', d2', atkr);
+
+   assert enc_conf_eqpdb(d1', d2', atkr);
+}
+
+predicate outside_world_same(d:PageDb, d':PageDb, p:PageNr, asp: PageNr) 
+    requires validPageDb(d) && validPageDb(d')
+    requires validPageNr(p) && valDispPage(d, p)
+    requires validPageNr(asp) && valAddrPage(d, asp)
+    requires d[p].addrspace == asp
+{
+    valDispPage(d', p) && valAddrPage(d', asp) && d'[p].addrspace == asp &&
+    (forall n : PageNr :: d'[n].PageDbEntryTyped? <==>
+        d[n].PageDbEntryTyped?) &&
+    (forall n : PageNr :: pgInAddrSpc(d', n, asp) <==>
+        pgInAddrSpc(d, n, asp)) &&
+    (forall n : PageNr | !pgInAddrSpc(d', n, asp) 
+        && d'[n].PageDbEntryTyped? ::
+            d'[n].addrspace == d[n].addrspace &&
+            d'[n].entry == d[n].entry)
+}
+
+lemma lemma_enter_only_affects_entered(s: state, d: PageDb, s': state, d': PageDb,
+                                       disp:PageNr, asp:PageNr, arg1: word, arg2: word, arg3: word)
+    requires ValidState(s) && validPageDb(d) && ValidState(s') && 
+        validPageDb(d') && SaneConstants()
+    requires validPageNr(disp) && valDispPage(d, disp)
+    requires validPageNr(asp) && valAddrPage(d, asp)
+    requires d[disp].addrspace == asp
+    requires smc_enter(s, d, s', d', disp, arg1, arg2, arg3)
+    requires smc_enter_err(d, disp, false) == KOM_ERR_SUCCESS
+    ensures outside_world_same(d, d', disp, asp)
+{
+    assume false;
+
+}
+
+
+predicate atkr_entry(d1: PageDb, d2: PageDb, disp: word, atkr: PageNr)
+{
+    validPageNr(disp) &&
+    validPageDb(d1) && validPageDb(d2) &&
+    valAddrPage(d1, atkr) && valAddrPage(d2, atkr) &&
+    d1[disp].PageDbEntryTyped? && d1[disp].entry.Dispatcher? &&
+    d2[disp].PageDbEntryTyped? && d2[disp].entry.Dispatcher? &&
+    nonStoppedDispatcher(d1, disp) && nonStoppedDispatcher(d2, disp) &&
+    d1[disp].addrspace == d2[disp].addrspace == atkr
+}
+
+lemma lemma_enter_enc_conf_atkr_enter(s1: state, d1: PageDb, s1':state, d1': PageDb,
+                                      s2: state, d2: PageDb, s2':state, d2': PageDb,
+                                      dispPage: word, arg1: word, arg2: word, arg3: word,
+                                      atkr: PageNr)
+    requires ni_reqs(s1, d1, s1', d1', s2, d2, s2', d2', atkr)
+    requires smc_enter(s1, d1, s1', d1', dispPage, arg1, arg2, arg3)
+    requires smc_enter(s2, d2, s2', d2', dispPage, arg1, arg2, arg3)
+    requires enc_conf_eqpdb(d1, d2, atkr)
+    requires entering_atkr(d1, d2, dispPage, atkr, false);
+    requires enc_conf_eq_entry(s1, s2, d1, d2, atkr)
+    ensures  enc_conf_eqpdb(d1', d2', atkr)
+    ensures  enc_conf_eq_entry(s1', s2', d1', d2', atkr)
+{
+
+    /*
+    var s11:state, steps1: nat :|
+        preEntryEnter(s1, s11, d1, dispPage, arg1, arg2, arg3) &&
+        validEnclaveExecution(s11, d1, s1', d1', dispPage, steps1);
+    
+    var s21:state, steps2: nat :|
+        preEntryEnter(s2, s21, d2, dispPage, arg1, arg2, arg3) &&
+        validEnclaveExecution(s21, d2, s2', d2', dispPage, steps2);
+
+    assert steps1 == steps2 by {
+        // TODO proveme :(
+        assume false;
+    }
+
+    var steps := steps1;
+    
+    lemma_validEnclaveEx_enc_conf(s11, d1, s1', d1', s21, d2, s2', d2',
+                                         dispPage, steps, atkr);
+    */
+
+    // TODO
+    // The thing that cannot be proven here is that the number of steps taken 
+    // is the same in both executions. Factor this out into a lemma.
+
+    forall(s11:state, s21:state, steps1:nat, steps2:nat |
+        preEntryEnter(s1, s11, d1, dispPage, arg1, arg2, arg3) &&
+        preEntryEnter(s2, s21, d2, dispPage, arg1, arg2, arg3) &&
+        validEnclaveExecution(s11, d1, s1', d1', dispPage, steps1) &&
+        validEnclaveExecution(s21, d2, s2', d2', dispPage, steps2))
+        ensures enc_conf_eqpdb(d1', d2', atkr)
+        ensures enc_conf_eq_entry(s1', s2', d1', d2', atkr)
+    {
+        assume steps1 == steps2;
+        assume s11.nd_public == s21.nd_public;
+        assume s11.nd_private == s21.nd_private;
+        lemma_validEnclaveEx_enc_conf(s11, d1, s1', d1', s21, d2, s2', d2',
+                                         dispPage, steps1, atkr);
+    }
+}
+
+lemma lemma_validEnclaveEx_enc_conf(s1: state, d1: PageDb, s1':state, d1': PageDb,
+                                    s2: state, d2: PageDb, s2':state, d2': PageDb,
+                                    dispPg: PageNr, steps:nat,
+                                    atkr: PageNr)
+    //requires ni_reqs(s1, d1, s1', d1', s2, d2, s2', d2', atkr)
+    requires ValidState(s1) && ValidState(s2) &&
+             ValidState(s1') && ValidState(s2') &&
+             validPageDb(d1) && validPageDb(d2) && 
+             validPageDb(d1') && validPageDb(d2') && SaneConstants()
+    requires atkr_entry(d1, d2, dispPg, atkr)
+    requires validEnclaveExecution(s1, d1, s1', d1', dispPg, steps)
+    requires validEnclaveExecution(s2, d2, s2', d2', dispPg, steps);
+    requires enc_conf_eqpdb(d1, d2, atkr)
+    requires enc_conf_eq_entry(s1, s2, d1, d2, atkr)
+    ensures  atkr_entry(d1', d2', dispPg, atkr)
+    ensures  enc_conf_eqpdb(d1', d2', atkr)
+    ensures  enc_conf_eq_entry(s1', s2', d1', d2', atkr)
+    decreases steps
+{
+    reveal_validEnclaveExecution();
+    var retToEnclave := (steps > 0);
+
+    // I can't figure out how to get around assuming nonStoppedDispatcher here. 
+    // I tried using a premium version of validEnclaveExecutionStep that calls 
+    // the lemma that proves nonstopped, but LHS values couldn't be found...
+
+    var s15, d15 :|
+        validEnclaveExecutionStep(s1, d1, s15, d15, dispPg, retToEnclave) &&
+        (if retToEnclave then
+            (assume nonStoppedDispatcher(d15, dispPg);
+            validEnclaveExecution(s15, d15, s1', d1', dispPg, steps - 1))
+          else
+             s1' == s15 && d1' == d15);
+
+    var s25, d25 :|
+        validEnclaveExecutionStep(s2, d2, s25, d25, dispPg, retToEnclave) &&
+        (if retToEnclave then 
+            (assume nonStoppedDispatcher(d25, dispPg);
+            validEnclaveExecution(s25, d25, s2', d2', dispPg, steps - 1))
+          else
+             s2' == s25 && d2' == d25);
+
+    lemma_validEnclaveExecutionStep_validPageDb(s1, d1, s15, d15, dispPg, retToEnclave);
+    lemma_validEnclaveExecutionStep_validPageDb(s2, d2, s25, d25, dispPg, retToEnclave);
+    lemma_validEnclaveStep_enc_conf(s1, d1, s15, d15, s2, d2, s25, d25,
+        dispPg, atkr, retToEnclave);
+
+    if(retToEnclave) {
+        lemma_validEnclaveExecution(s15, d15, s1', d1', dispPg, steps - 1);
+        lemma_validEnclaveExecution(s25, d25, s2', d2', dispPg, steps - 1);
+        lemma_validEnclaveEx_enc_conf(s15, d15, s1', d1', s25, d25, s2', d2',
+                                         dispPg, steps -1, atkr);
+        assert enc_conf_eqpdb(d1', d2', atkr);
+        assert enc_conf_eq_entry(s1', s2', d1', d2', atkr);
+    } else {
+        assert s2' == s25;
+        assert s1' == s15;
+        assert d1' == d15;
+        assert d2' == d25;
+        assert enc_conf_eqpdb(d1', d2', atkr);
+        assert enc_conf_eq_entry(s1', s2', d1', d2', atkr);
+    }
+}
+
+lemma lemma_validEnclaveStep_enc_conf(s1: state, d1: PageDb, s1':state, d1': PageDb,
+                                      s2: state, d2: PageDb, s2':state, d2': PageDb,
+                                      dispPage:PageNr, atkr: PageNr, ret:bool)
+    requires ValidState(s1) && ValidState(s2) &&
+             ValidState(s1') && ValidState(s2') &&
+             validPageDb(d1) && validPageDb(d2) && 
+             validPageDb(d1') && validPageDb(d2') && SaneConstants()
+    requires atkr_entry(d1, d2, dispPage, atkr)
+    requires validEnclaveExecutionStep(s1, d1, s1', d1', dispPage, ret);
+    requires validEnclaveExecutionStep(s2, d2, s2', d2', dispPage, ret);
+    requires enc_conf_eqpdb(d1, d2, atkr)
+    requires enc_conf_eq_entry(s1, s2, d1, d2, atkr)
+    ensures  atkr_entry(d1', d2', dispPage, atkr)
+    ensures  enc_conf_eqpdb(d1', d2', atkr)
+    ensures  enc_conf_eq_entry(s1', s2', d1', d2', atkr)
+{
+    assume false;
+    // use lemma below...
+    //
+    // I'm guessing that even with the lemma below, this will be just as 
+    // annoying as the above lemma
+}
+
+lemma lemma_validEnclaveStepPrime_enc_conf(
+s11: state, d11: PageDb, s12:state, s13:state, s14:state, d14:PageDb,
+r1:state, rd1:PageDb,
+s21: state, d21: PageDb, s22:state, s23:state, s24:state, d24:PageDb,
+r2:state, rd2:PageDb,
+dispPg:PageNr, retToEnclave:bool, atkr: PageNr
+)
+    requires ValidState(s11) && ValidState(s21) &&
+             ValidState(r1)  && ValidState(r2)  &&
+             validPageDb(d11) && validPageDb(d21) &&
+             validPageDb(rd1) && validPageDb(rd2) && SaneConstants()
+    requires atkr_entry(d11, d21, dispPg, atkr)
+    requires validEnclaveExecutionStep'(s11,d11,s12,s13,s14,d14,r1,rd1,dispPg,retToEnclave)
+    requires validEnclaveExecutionStep'(s21,d21,s22,s23,s24,d24,r2,rd2,dispPg,retToEnclave)
+    requires enc_conf_eqpdb(d11, d21, atkr)
+    requires enc_conf_eq_entry(s11, s21, d11, d21, atkr)
+    ensures  atkr_entry(rd1, rd2, dispPg, atkr)
+    ensures  enc_conf_eqpdb(rd1, rd2, atkr)
+    ensures  enc_conf_eq_entry(r1, r2, rd1, rd2, atkr)
+{
+
+    assert l1pOfDispatcher(d11, dispPg) == l1pOfDispatcher(d21, dispPg) by
+        { reveal_enc_conf_eqpdb(); }
+    var l1p := l1pOfDispatcher(d11, dispPg);
+
+    assert s12.m == s11.m;
+    assert s22.m == s21.m;
+    assert dataPagesCorrespond(s11.m, d11);
+    assert dataPagesCorrespond(s21.m, d21);
+    
+    assert userspaceExecutionAndException(s12, s13, s14);
+    assert userspaceExecutionAndException(s22, s23, s24);
+
+    assert pageTableCorresponds(s12, d11, l1p) by
+    { 
+        assert pageTableCorresponds(s11, d11, l1p);
+        reveal pageTableCorresponds();
+    }
+
+    assert pageTableCorresponds(s22, d21, l1p) by
+    { 
+        assert pageTableCorresponds(s21, d21, l1p);
+        reveal pageTableCorresponds();
+    }
+
+    // avoid proving anything about nd sources...
+    assert enc_conf_eq_entry(s12, s22, d11, d21, atkr) by
+    {
+        assume s22.nd_private == s12.nd_private;
+        assume s22.nd_public  == s12.nd_public;
+    }
+
+    lemma_userspaceExec_atkr_conf(s12, s13, d11, s22, s23, d21, dispPg, atkr);
+
+    assert d14 == d24;
+
+    // TODO proveme
+    assume isReturningSvc(s14) == isReturningSvc(s24);
+
+    if(isReturningSvc(s14)) {
+        assert rd1 == d14;
+        assert rd2 == d24;
+        reveal_enc_conf_eqpdb();
+        assert rd1 == rd2;
+        assert enc_conf_eqpdb(rd1, rd2, atkr);
+        // avoid proving anything about nd sources...
+        assume enc_conf_eq_entry(r1, r2, rd1, rd2, atkr);
+    } else {
+        assume false; 
+    }
+
+
+    // Half-baked proof-sketch that will be split into a bunch of lemmas:
+    // if s13 ~ d11 && s23 ~ d21 &&
+    //      conf_eq(d11, d21) &&
+    //      s13.nd == s23.d 
+    // then:
+    //      forall s14, s24:
+    //      updatePagesFromState(s13, d11, s14) ==
+    //      updatePagesFromState(s23, d21, s24) 
+    //
+    // by:
+    //
+    // forall p :: pgSWrInAsp(d11, p, l1p) <==> pgSWrInAsp(d21, p, l1p)
+    // (should follow from conf_eq(d1, d2) and l1p is the attacker's)
+    //
+    // updateUserPage(s13, d11, p) == updateUserPage(s23, d21, p)
+    //          by:
+    //              - s13.nd == s23.nd
+    //              - (r1.nd == r2.nd && excpt(r1, r1') && excpt(r2, r2') ==>
+    //                  r1'.nd == r2'.nd)
+    //              - def of evalUserspace (esp. havoc)
+    //              - writable pages same
+    //                  by: s13 ~ d11 && s23 ~d21 &&
+    //                      conf_eq(d11, d21) &&
+    //                      l1p == atkr.l1p
+    //              - contents written same (by s13.nd == s23.nd)
+    //
+    //
+    assume false;
+}
+
+lemma lemma_userspaceExec_atkr_conf(
+s12: state, s13:state, d1:PageDb,
+s22: state, s23:state, d2:PageDb,
+dispPg: PageNr, atkr: PageNr)
+    requires ValidState(s12) && ValidState(s22) &&
+             validPageDb(d1) && validPageDb(d2) && SaneConstants()
+    requires enc_conf_eq_entry(s12, s22, d1, d2, atkr);
+    requires evalUserspaceExecution(s12, s13)
+    requires evalUserspaceExecution(s22, s23)
+    requires atkr_entry(d1, d2, dispPg, atkr)
+    requires enc_conf_eqpdb(d1, d2, atkr)
+    requires l1pOfDispatcher(d1, dispPg) == l1pOfDispatcher(d2, dispPg);
+    requires (var l1p := l1pOfDispatcher(d1, dispPg);
+        pageTableCorresponds(s12, d1, l1p) &&
+        pageTableCorresponds(s22, d2, l1p) &&
+        dataPagesCorrespond(s12.m, d1) &&
+        dataPagesCorrespond(s22.m, d2))
+    ensures (var d14 := updateUserPagesFromState(s13, d1, dispPg);
+        var d24 := updateUserPagesFromState(s23, d2, dispPg);
+        d14 == d24 && d14[atkr].PageDbEntryTyped? &&
+            d24[atkr].PageDbEntryTyped? &&
+            valAddrPage(d14, atkr) && valAddrPage(d24, atkr))
+{
+   assume false;
+
+
+}
+
+
+//-----------------------------------------------------------------------------
+// Resume
+//-----------------------------------------------------------------------------
+lemma lemma_resume_enc_conf_ni(s1: state, d1: PageDb, s1':state, d1': PageDb,
+                               s2: state, d2: PageDb, s2':state, d2': PageDb,
+                               dispPage: word,
+                               atkr: PageNr)
+    requires ni_reqs(s1, d1, s1', d1', s2, d2, s2', d2', atkr)
+    requires smc_resume(s1, d1, s1', d1', dispPage)
+    requires smc_resume(s2, d2, s2', d2', dispPage)
+    requires enc_conf_eqpdb(d1, d2, atkr)
+    requires entering_atkr(d1, d2, dispPage, atkr, true) ==>
+        enc_conf_eq_entry(s1, s2, d1, d2, atkr)
+    ensures enc_conf_eqpdb(d1', d2', atkr)
+    ensures entering_atkr(d1, d2, dispPage, atkr, true) ==>
+        enc_conf_eq_entry(s1', s2', d1', d2', atkr)
+{
+    // TODO proveme
+    assume false;
+}
