verified/sec_prop_util.i.dfy
@@ -1,0 +1,68 @@
+include "sec_prop.s.dfy"
+include "pagedb.s.dfy"
+include "entry.s.dfy"
+include "sec_prop_util.i.dfy"
+
+predicate ni_reqs(s1: state, d1: PageDb, s1': state, d1': PageDb,
+                  s2: state, d2: PageDb, s2': state, d2': PageDb,
+                  atkr: PageNr)
+{
+    ValidState(s1) && ValidState(s1') && 
+    ValidState(s2) && ValidState(s2') &&
+    SaneConstants() &&
+    validPageDb(d1) && validPageDb(d1') &&
+    validPageDb(d2) && validPageDb(d2') &&
+    valAddrPage(d1, atkr) && valAddrPage(d2, atkr) &&
+    (forall n : PageNr :: d1[n].PageDbEntryFree? <==> d2[n].PageDbEntryFree?)
+    /*
+    SaneState(s1) && validPageDb(d1) && SaneState(s1') && validPageDb(d1') &&
+    SaneState(s2) && validPageDb(d2) && SaneState(s2') && validPageDb(d2') &&
+    pageDbCorresponds(s1.m, d1) && pageDbCorresponds(s1'.m, d1') &&
+    pageDbCorresponds(s2.m, d2) && pageDbCorresponds(s2'.m, d2') &&
+    valAddrPage(d1, atkr) && valAddrPage(d2, atkr) &&
+    (forall n : PageNr :: d1[n].PageDbEntryFree? <==> d2[n].PageDbEntryFree?)
+    */
+}
+
+predicate ni_reqs_(d1: PageDb, d1': PageDb, d2: PageDb, d2': PageDb, atkr: PageNr)
+{
+    validPageDb(d1) && validPageDb(d1') &&
+    validPageDb(d2) && validPageDb(d2') &&
+    valAddrPage(d1, atkr) && valAddrPage(d2, atkr) &&
+    // This is a slight weakening of the security property...
+    (forall n : PageNr :: d1[n].PageDbEntryFree? <==> d2[n].PageDbEntryFree?)
+}
+
+// Note, the proofs seem to go faster if I don't just reference ni_reqs_weak_ 
+// in ni_reqs_
+predicate ni_reqs_weak_(d1: PageDb, d1': PageDb, d2: PageDb, d2': PageDb, atkr: PageNr)
+{
+    validPageDb(d1) && validPageDb(d1') &&
+    validPageDb(d2) && validPageDb(d2') &&
+    valAddrPage(d1, atkr) && valAddrPage(d2, atkr)
+}
+
+predicate same_call_args(s1:state, s2: state)
+    requires ValidState(s1) && ValidState(s2)
+{
+    reveal_ValidRegState();
+    reveal_ValidSRegState();
+    OperandContents(s1, OReg(R0))  == OperandContents(s2, OReg(R0)) &&
+    OperandContents(s1, OReg(R1))  == OperandContents(s2, OReg(R1)) &&
+    OperandContents(s1, OReg(R2))  == OperandContents(s2, OReg(R2)) &&
+    OperandContents(s1, OReg(R3))  == OperandContents(s2, OReg(R3)) &&
+    OperandContents(s1, OReg(R4))  == OperandContents(s2, OReg(R4))
+}
+
+predicate entering_atkr(d1: PageDb, d2: PageDb, disp: word, atkr: PageNr, is_resume:bool)
+    requires validPageDb(d1) && validPageDb(d2)
+    requires valAddrPage(d1, atkr) && valAddrPage(d2, atkr)
+{
+    validPageNr(disp) &&
+    d1[disp].PageDbEntryTyped? && d1[disp].entry.Dispatcher? &&
+    d2[disp].PageDbEntryTyped? && d2[disp].entry.Dispatcher? &&
+    d1[disp].addrspace == atkr && d2[disp].addrspace == atkr &&
+    nonStoppedDispatcher(d1, disp) && nonStoppedDispatcher(d2, disp) &&
+    smc_enter_err(d1, disp, is_resume) == KOM_ERR_SUCCESS &&
+    smc_enter_err(d2, disp, is_resume) == KOM_ERR_SUCCESS
+}
